src/tls/FFI.fst
@@ -298,6 +298,16 @@ let ffiSetNamedGroups cfg x =
   namedGroups = ngl
   }
 
+val ffiSetALPN: cfg:config -> x:string -> ML config
+let ffiSetALPN cfg x =
+  let apl = String.split [':'] x in
+  if List.Tot.length apl > 255 then failwith "ffiSetALPN: too many entries";
+  let apl = List.map (fun x ->
+    if String.length x < 256 then x
+    else failwith ("ffiSetALPN: protocol <"^x^"> is too long")
+  ) apl in
+  { cfg with alpn = Some apl }
+
 val ffiSetTicketKey: x:string -> ML bool
 let ffiSetTicketKey x =
   match String.split [':'] x with
